rework spmv

dafny/spmv.dfy
@@ -1,3 +1,4 @@
+<<<<<<< HEAD
 function sum(vals: array<int>, crd: array<nat>, x : array<int>, b : int, k : int) : (s : int)
   reads vals, crd, x
   requires b >= 0
@@ -39,10 +40,51 @@ method SpMV(vals: array<int>, crd: array<nat>, pos: array<nat>, x : array<int>) 
           invariant idx <= pos[row + 1]
           invariant forall i :: 0 <= i < row ==> y[i] == sum(vals, crd, x, pos[i], pos[i + 1])
           invariant y[row] == sum(vals, crd, x, pos[row], idx) 
+=======
+function sum(X_val: array<int>, X_crd: array<nat>, v : array<int>, b : int, k : int) : (s : int)
+  reads X_val, X_crd, v
+  requires X_val.Length >= b >= 0
+  requires k <= X_val.Length
+  requires X_val.Length == X_crd.Length
+  requires forall i :: 0 <= i < X_crd.Length ==> 0 <= X_crd[i] < v.Length
+  ensures k <= b ==> s == 0
+  ensures b < k ==> s ==  sum(X_val, X_crd, v, b + 1, k) + X_val[b] * v[X_crd[b]]
+  decreases k - b
+  {
+    if k <= b then 
+      0
+    else  sum(X_val, X_crd, v, b + 1, k) + X_val[b] * v[X_crd[b]]
+  }
+
+
+method SpMV(X_val: array<int>, X_crd: array<nat>, X_pos: array<nat>, v : array<int>) returns (y : array<int>)
+  requires X_crd.Length >= 1 
+  requires X_crd.Length == X_val.Length;
+  requires forall i, j :: 0 <= i < j < X_pos.Length ==> X_pos[i] <= X_pos[j];
+  requires forall i :: 0 <= i < X_crd.Length ==> X_crd[i] < v.Length
+  requires forall i :: 0 <= i < X_pos.Length ==> X_pos[i] <= X_val.Length
+  requires X_pos.Length >= 1
+  ensures y.Length + 1 == X_pos.Length
+  ensures forall i :: 0 <= i < y.Length ==> y[i] == sum(X_val, X_crd, v, X_pos[i], X_pos[i + 1])
+  {
+    var N: nat := X_pos.Length - 1;
+    y := new int[N];
+    var n: nat := 0;
+    while n < N
+      invariant n <= y.Length
+      invariant forall i :: 0 <= i < n ==> y[i] == sum(X_val, X_crd, v, X_pos[i], X_pos[i + 1])
+      { 
+        y[n] := 0;
+        var k: nat := X_pos[n];
+        while k < X_pos[n + 1]
+          invariant k <= X_pos[n + 1]
+          invariant forall i :: 0 <= i < n ==> y[i] == sum(X_val, X_crd, v, X_pos[i], X_pos[i + 1])
+          invariant y[n] + sum(X_val, X_crd, v, k, X_pos[n+1]) == sum(X_val, X_crd, v, X_pos[n], X_pos[n+1]) 
+>>>>>>> 8ef3df9 (rework spmv)
           {
-            y[row] := y[row] + vals[idx] * x[crd[idx]];
-            idx := idx + 1;
+            y[n] := y[n] + X_val[k] * v[X_crd[k]];
+            k := k + 1;
           }
-        row := row + 1;
+        n := n + 1;
       }
   }
